mark-and-sweep/spec/GC.Spec.ChunkedMajorGC.Graph.fsti
@@ -126,6 +126,20 @@ val chunked_major_field_data_preserved_intro
             MarkDefs.chunked_get_field mh_final x i))
       (ensures chunked_major_field_data_preserved mh_init mh_final x)
 
+val chunked_major_field_data_preserved_elim
+  (mh_init: MH.major_heap)
+  (mh_final: MH.major_heap)
+  (x: obj_addr)
+  : Lemma
+      (requires chunked_major_field_data_preserved mh_init mh_final x)
+      (ensures
+       chunked_major_vertex mh_init x /\
+       chunked_major_vertex mh_final x /\
+       (forall (i: U64.t). U64.v i >= 1 /\
+         U64.v i <= U64.v (SweepDefs.chunked_wosize_of_object mh_init x) ==>
+         MarkDefs.chunked_get_field mh_init x i ==
+           MarkDefs.chunked_get_field mh_final x i))
+
 val chunked_major_live_subgraph_vertices_elim
   (mh_init: MH.major_heap)
   (mh_final: MH.major_heap)
